proof/theories/Optimizer/Optimize_ConcatGuarded.v
@@ -192,44 +192,6 @@ Qed.
 
 (** ** Loadability / outcome / applies of the guarded shells. *)
 
-Lemma orig_rule2g_applies : forall f1 f2 gm a b body r1 e p,
-  rule_applies (orig_rule2g f1 f2 gm a b body r1) e p
-  = andb (andb (andb (eval_matchcond (MCmp f1 CEq a) e p) (eval_matchcond gm e p))
-               (eval_matchcond (MCmp f2 CEq b) e p))
-         (rule_applies_walk body e p).
-Proof.
-  intros. unfold orig_rule2g. rewrite rule_applies_mk_head.
-  cbn [rule_applies_walk]. rewrite !Bool.andb_assoc. reflexivity.
-Qed.
-
-Lemma merged_rule2g_loadable_eq_orig : forall f1 f2 gm name a b body r1 e p,
-  rule_loadable (merged_rule2g f1 f2 gm name body r1) e p
-  = rule_loadable (orig_rule2g f1 f2 gm a b body r1) e p.
-Proof.
-  intros. unfold merged_rule2g, orig_rule2g. rewrite !rule_loadable_mk_head.
-  rewrite !synproxy_stops_bmatch, !body_thread_bmatch.
-  cbn [body_loadable_walk body_item_loadable match_loadable fields_loadable forallb].
-  rewrite Bool.andb_true_r. btauto.
-Qed.
-
-Lemma merged_rule2g_outcome_eq_orig : forall f1 f2 gm name a b body r1 e p,
-  outcome (merged_rule2g f1 f2 gm name body r1) e p
-  = outcome (orig_rule2g f1 f2 gm a b body r1) e p.
-Proof.
-  intros. unfold merged_rule2g, orig_rule2g. rewrite !outcome_mk_head.
-  rewrite !synproxy_stops_bmatch, !body_thread_bmatch. reflexivity.
-Qed.
-
-Lemma merged_rule2g_applies : forall f1 f2 gm name body r1 e p,
-  rule_applies (merged_rule2g f1 f2 gm name body r1) e p
-  = andb (eval_matchcond gm e p)
-         (andb (eval_matchcond (MConcatSet [f1; f2] false name) e p)
-               (rule_applies_walk body e p)).
-Proof.
-  intros. unfold merged_rule2g. rewrite rule_applies_mk_head.
-  cbn [rule_applies_walk]. reflexivity.
-Qed.
-
 (** The guard factors out of the [existsb] over the run. *)
 Lemma existsb_guard_factor : forall (A : Type) (c1 c2 : A -> bool) (G W : bool) (l : list A),
   existsb (fun x => andb (andb (andb (c1 x) G) (c2 x)) W) l
